src/DY.Example.NSL.SecurityProperties.fst
@@ -21,8 +21,7 @@ val initiator_authentication:
     principal_corrupt tr alice \/ principal_corrupt tr bob \/
     event_triggered (prefix tr i) alice nsl_event_label (serialize nsl_event (Initiate2 alice bob n_a n_b))
   )
-let initiator_authentication tr i alice bob n_a n_b =
-  parse_serialize_inv_lemma #bytes nsl_event (Respond2 alice bob n_a n_b)
+let initiator_authentication tr i alice bob n_a n_b = ()
 
 val responder_authentication:
   tr:trace -> i:nat ->
@@ -36,9 +35,9 @@ val responder_authentication:
     principal_corrupt tr alice \/ principal_corrupt tr bob \/
     event_triggered (prefix tr i) bob nsl_event_label (serialize nsl_event (Respond1 alice bob n_a n_b))
   )
-let responder_authentication tr i alice bob n_a n_b =
-  parse_serialize_inv_lemma #bytes nsl_event (Initiate2 alice bob n_a n_b)
+let responder_authentication tr i alice bob n_a n_b = ()
 
+#push-options "--z3rlimit 50"
 val n_a_secrecy:
   tr:trace -> alice:principal -> bob:principal -> n_a:bytes ->
   Lemma
@@ -53,21 +52,13 @@ val n_a_secrecy:
   (ensures principal_corrupt tr alice \/ principal_corrupt tr bob)
 let n_a_secrecy tr alice bob n_a =
   attacker_only_knows_publishable_values nsl_protocol_preds tr n_a;
-  introduce (exists sess_id. typed_state_was_set tr nsl_session_label alice sess_id (InitiatorSentMsg1 bob n_a <: nsl_session)) ==> (principal_corrupt tr alice \/ principal_corrupt tr bob) with _. (
-    parse_serialize_inv_lemma #bytes nsl_event (Initiate1 alice bob n_a)
-  );
   introduce (exists sess_id n_b. typed_state_was_set tr nsl_session_label alice sess_id (InitiatorSentMsg3 bob n_a n_b <: nsl_session)) ==> (principal_corrupt tr alice \/ principal_corrupt tr bob) with _. (
     eliminate exists sess_id n_b. typed_state_was_set tr nsl_session_label alice sess_id (InitiatorSentMsg3 bob n_a n_b <: nsl_session) returns _ with _. (
-      parse_serialize_inv_lemma #bytes nsl_event (Initiate2 alice bob n_a n_b);
-      parse_serialize_inv_lemma #bytes nsl_event (Initiate1 alice bob n_a);
       assert(event_triggered tr alice nsl_event_label (serialize nsl_event (Initiate1 alice bob n_a)))
     )
   );
   introduce (exists sess_id n_b. typed_state_was_set tr nsl_session_label bob sess_id (ResponderReceivedMsg3 alice n_a n_b <: nsl_session)) ==> (principal_corrupt tr alice \/ principal_corrupt tr bob) with _. (
     eliminate exists sess_id n_b. typed_state_was_set tr nsl_session_label bob sess_id (ResponderReceivedMsg3 alice n_a n_b <: nsl_session) returns _ with _. (
-      parse_serialize_inv_lemma #bytes nsl_event (Respond2 alice bob n_a n_b);
-      parse_serialize_inv_lemma #bytes nsl_event (Initiate2 alice bob n_a n_b);
-      parse_serialize_inv_lemma #bytes nsl_event (Initiate1 alice bob n_a);
       assert(
         principal_corrupt tr alice \/ principal_corrupt tr bob \/
         event_triggered tr alice nsl_event_label (serialize nsl_event (Initiate2 alice bob n_a n_b))
@@ -78,6 +69,7 @@ let n_a_secrecy tr alice bob n_a =
       )
     )
   )
+#pop-options
 
 val n_b_secrecy:
   tr:trace -> alice:principal -> bob:principal -> n_b:bytes ->
@@ -93,22 +85,13 @@ val n_b_secrecy:
   (ensures principal_corrupt tr alice \/ principal_corrupt tr bob)
 let n_b_secrecy tr alice bob n_b =
   attacker_only_knows_publishable_values nsl_protocol_preds tr n_b;
-  introduce (exists sess_id n_a. typed_state_was_set tr nsl_session_label bob sess_id (ResponderSentMsg2 alice n_a n_b <: nsl_session)) ==> (principal_corrupt tr alice \/ principal_corrupt tr bob) with _. (
-    eliminate exists sess_id n_a. typed_state_was_set tr nsl_session_label bob sess_id (ResponderSentMsg2 alice n_a n_b <: nsl_session) returns _ with _. (
-      parse_serialize_inv_lemma #bytes nsl_event (Respond1 alice bob n_a n_b)
-    )
-  );
   introduce (exists sess_id n_a. typed_state_was_set tr nsl_session_label bob sess_id (ResponderReceivedMsg3 alice n_a n_b <: nsl_session)) ==> (principal_corrupt tr alice \/ principal_corrupt tr bob) with _. (
     eliminate exists sess_id n_a. typed_state_was_set tr nsl_session_label bob sess_id (ResponderReceivedMsg3 alice n_a n_b <: nsl_session) returns _ with _. (
-      parse_serialize_inv_lemma #bytes nsl_event (Respond2 alice bob n_a n_b);
-      parse_serialize_inv_lemma #bytes nsl_event (Respond1 alice bob n_a n_b);
       assert(event_triggered tr bob nsl_event_label (serialize nsl_event (Respond1 alice bob n_a n_b)))
     )
   );
   introduce (exists sess_id n_a. typed_state_was_set tr nsl_session_label alice sess_id (InitiatorSentMsg3 bob n_a n_b <: nsl_session)) ==> (principal_corrupt tr alice \/ principal_corrupt tr bob) with _. (
     eliminate exists sess_id n_a. typed_state_was_set tr nsl_session_label alice sess_id (InitiatorSentMsg3 bob n_a n_b <: nsl_session) returns _ with _. (
-      parse_serialize_inv_lemma #bytes nsl_event (Initiate2 alice bob n_a n_b);
-      parse_serialize_inv_lemma #bytes nsl_event (Respond1 alice bob n_a n_b);
       assert(
         principal_corrupt tr alice \/ principal_corrupt tr bob \/
         event_triggered tr bob nsl_event_label (serialize nsl_event (Respond1 alice bob n_a n_b))
